ulib/LowStar.Monotonic.Buffer.fsti
@@ -1,0 +1,304 @@
+module LowStar.Monotonic.Buffer
+
+module P = FStar.Preorder
+module G = FStar.Ghost
+module U32 = FStar.UInt32
+module Seq = FStar.Seq
+
+module HS = FStar.HyperStack
+module HST = FStar.HyperStack.ST
+
+(* Most comments are taken from the Low* tutorial at:
+   https://fstarlang.github.io/lowstar/html/LowStar.html
+ *)
+
+(* Shorthand for preorder over sequences *)
+type srel (a:Type0) = P.preorder (Seq.seq a)
+
+
+/// Low* buffers
+/// ==============
+///
+/// The workhorse of Low*, this module allows modeling C arrays on the
+/// stack and in the heap.  At compilation time, KreMLin implements
+/// buffers using C arrays, i.e. if Low* type ``t`` is translated into C
+/// type ``u``, then Low* type ``buffer t`` is translated to C type ``u*``.
+///
+/// The type is indexed by two preorders:
+/// rrel is the starting preorder with which the original buffer was initially created
+/// rel  is the preorder of the current buffer (which could be a sub-buffer of the original one)
+///
+/// The buffer contents are constrained to evolve according to rel
+
+val mbuffer (a:Type0) (rrel rel:srel a) :Tot Type0
+
+/// The C ``NULL`` pointer is represented as the Low* ``null`` buffer. For
+/// any given type, there is exactly one ``null`` buffer of this type,
+/// just like there is exactly one C ``NULL`` pointer of any given type.
+///
+/// The nullity test ``g_is_null`` is ghost, for proof purposes
+/// only. The corresponding stateful nullity test is ``is_null``, see
+/// below.
+
+(* FIXME: The nullity test for proof purposes is currently expressed
+   as a ghost predicate, `g_is_null`, but it is scheduled to be
+   replaced with equality with `null` *)
+
+val g_is_null (#a:Type0) (#rrel #rel:srel a) (b:mbuffer a rrel rel) :GTot bool
+
+val null (#a:Type0) (#rrel #rel:srel a) :Tot (b:mbuffer a rrel rel {g_is_null b})
+
+val null_unique (#a:Type0) (#rrel #rel:srel a) (b:mbuffer a rrel rel) :Lemma (g_is_null b <==> b == null)
+
+/// ``unused_in b h`` holds only if buffer ``b`` has not been allocated
+/// yet.
+
+val unused_in (#a:Type0) (#rrel #rel:srel a) (b:mbuffer a rrel rel) (h:HS.mem) :GTot Type0
+
+
+/// ``live h b`` holds if, and only if, buffer ``b`` is currently
+/// allocated in ``h`` and has not been deallocated yet.
+///
+/// This predicate corresponds to the C notion of "lifetime", and as
+/// such, is a prerequisite for all stateful operations on buffers
+/// (see below), per the C standard:
+///
+///   If an object is referred to outside of its lifetime, the
+///   behavior is undefined.
+/// 
+///   -- ISO/IEC 9899:2011, Section 6.2.4 paragraph 2
+/// 
+/// By contrast, it is not required for the ghost versions of those
+/// operators.
+
+val live (#a:Type0) (#rrel #rel:srel a) (h:HS.mem) (b:mbuffer a rrel rel) :GTot Type0
+
+
+/// The null pointer is always live.
+
+val live_null (a:Type0) (rrel rel:srel a) (h:HS.mem) :Lemma (live h (null #a #rrel #rel))
+
+let live_is_null (#a:Type0) (#rrel #rel:srel a) (h:HS.mem) (b:mbuffer a rrel rel)
+  :Lemma (requires (g_is_null b == true))
+         (ensures (live h b))
+         [SMTPat (live h b)]
+  = null_unique b;
+    live_null a rrel rel h
+
+/// A live buffer has already been allocated.
+
+val live_not_unused_in (#a:Type0) (#rrel #rel:srel a) (h:HS.mem) (b:mbuffer a rrel rel)
+  :Lemma (requires (live h b /\ b `unused_in` h)) (ensures False)
+
+
+(* FIXME: the following definition is necessary to isolate the pattern
+   because of unification. In other words, if we attached the pattern
+   to `live_not_unused_in`, then we would not be able to use
+   `FStar.Classical.forall_intro_`n and
+   `FStar.Classical.move_requires` due to unification issues.  Anyway,
+   we plan to isolate patterns in a separate module to clean up the Z3
+   context.
+ *)
+
+let live_not_unused_in' (#a:Type0) (#rrel #rel:srel a) (h:HS.mem) (b:mbuffer a rrel rel)
+  :Lemma (requires (live h b /\ b `unused_in` h))
+         (ensures False)
+         [SMTPat (live h b); SMTPat (b `unused_in` h)]
+  = live_not_unused_in h b
+
+
+/// Buffers live in the HyperStack model, which is an extension of
+/// the HyperHeap model, a hierarchical memory model that divides the
+/// heap into a tree of regions. This coarse-grained separation
+/// allows the programmer to state modifies clauses at the level of
+/// regions, rather than on individual buffers.
+///
+/// The HyperHeap memory model is described:
+///  - in the 2016 POPL paper: https://www.fstar-lang.org/papers/mumon/
+///  - in the relevant section of the F* tutorial: http://www.fstar-lang.org/tutorial/
+///
+/// ``frameOf b`` returns the identifier of the region in which the
+/// buffer ``b`` lives.
+
+val frameOf (#a:Type0) (#rrel #rel:srel a) (b:mbuffer a rrel rel) :Tot HS.rid
+
+
+/// ``as_addr b`` returns the abstract address of the buffer in its
+/// region, as an allocation unit: two buffers that are allocated
+/// separately in the same region will actually have different
+/// addresses, but a sub-buffer of a buffer will actually have the
+/// same address as its enclosing buffer.
+
+val as_addr (#a:Type0) (#rrel #rel:srel a) (b:mbuffer a rrel rel) :GTot nat
+
+
+/// A buffer is unused if, and only if, its address is unused.
+
+val unused_in_equiv (#a:Type0) (#rrel #rel:srel a) (b:mbuffer a rrel rel) (h:HS.mem)
+  :Lemma (unused_in b h <==>
+          (HS.live_region h (frameOf b) ==> as_addr b `Heap.addr_unused_in` (Map.sel (HS.get_hmap h) (frameOf b))))
+
+
+/// If a buffer is live, then so is its region.
+
+val live_region_frameOf (#a:Type0) (#rrel #rel:srel a) (h:HS.mem) (b:mbuffer a rrel rel)
+  :Lemma (requires (live h b))
+         (ensures (HS.live_region h (frameOf b)))
+         [SMTPatOr [
+	     [SMTPat (live h b)];
+             [SMTPat (HS.live_region h (frameOf b))];
+         ]]
+
+
+/// The length of a buffer ``b`` is available as a machine integer ``len
+/// b`` or as a mathematical integer ``length b``, but both in ghost
+/// (proof) code only: just like in C, one cannot compute the length
+/// of a buffer at run-time.
+
+val len (#a:Type0) (#rrel #rel:srel a) (b:mbuffer a rrel rel) :GTot U32.t
+
+let length (#a:Type0) (#rrel #rel:srel a) (b:mbuffer a rrel rel) :GTot nat = U32.v (len b)
+
+
+/// The null pointer has length 0.
+
+val len_null (a:Type0) (rrel rel:srel a) :Lemma (len (null #a #rrel #rel) == 0ul)
+
+let length_null_1 (#a:Type0) (#rrel #rel:srel a) (b:mbuffer a rrel rel)
+  :Lemma (requires (length b =!= 0)) (ensures (g_is_null b == false))
+         [SMTPat (length b)]
+  = len_null a rrel rel;
+    null_unique b
+
+let length_null_2 (#a:Type0) (#rrel #rel:srel a) (b:mbuffer a rrel rel)
+  :Lemma (requires (g_is_null b == true)) (ensures (length b == 0))
+         [SMTPat (g_is_null b)]
+  = len_null a rrel rel;
+    null_unique b
+
+
+/// For functional correctness, buffers are reflected at the proof
+/// level using sequences, via ``as_seq b h``, which returns the
+/// contents of a given buffer ``b`` in a given heap ``h``. If ``b`` is not
+/// live in ``h``, then the result is unspecified.
+
+(* TODO: why not return a lseq and remove length_as_seq lemma? *)
+val as_seq (#a:Type0) (#rrel #rel:srel a) (h:HS.mem) (b:mbuffer a rrel rel) :GTot (Seq.seq a)
+
+
+/// The contents of a buffer ``b`` has the same length as ``b`` itself.
+
+val length_as_seq (#a:Type0) (#rrel #rel:srel a) (h:HS.mem) (b:mbuffer a rrel rel)
+  :Lemma (Seq.length (as_seq h b) == length b)
+         [SMTPat (Seq.length (as_seq h b))]
+
+
+/// ``get`` is an often-convenient shorthand to index the value of a
+/// given buffer in a given heap, for proof purposes.
+
+
+let get (#a:Type0) (#rrel #rel:srel a) (h:HS.mem) (p:mbuffer a rrel rel) (i:nat)
+  :Ghost a (requires (i < length p)) (ensures (fun _ -> True))
+  = Seq.index (as_seq h p) i
+
+/// Before defining sub-buffer related API, we need to define the notion of "compatibility"
+///
+/// Sub-buffers can be taken at a different preorder than their parent buffers
+/// But it is subject to the following compatibility relation:
+///
+/// The main idea is to ensure that any modifications to the parent buffer are compatible with the sub-buffer preorder
+/// and vice-versa
+
+let compatible_sub_preorder (#a:Type0)
+  (len:nat) (pre:srel a)
+  (offset:nat) (sub_len:nat{offset + sub_len <= len}) (sub_pre:srel a)
+  = (forall (s1 s2:Seq.seq a). (Seq.length s1 == len /\ Seq.length s2 == len /\ pre s1 s2) ==>
+		          (sub_pre (Seq.slice s1 offset (offset + sub_len))
+			           (Seq.slice s2 offset (offset + sub_len)))) /\
+    (forall (s s2:Seq.seq a). (Seq.length s == len /\ Seq.length s2 == sub_len /\ sub_pre (Seq.slice s offset (offset + sub_len)) s2) ==>
+  		         (pre s (replace_subseq s offset sub_len s2)))
+
+/// ``gsub`` is the way to carve a sub-buffer out of a given
+/// buffer. ``gsub b i len`` return the sub-buffer of ``b`` starting from
+/// offset ``i`` within ``b``, and with length ``len``. Of course ``i`` and
+/// ``len`` must fit within the length of ``b``.
+///
+/// ``gsub`` is the ghost version, for proof purposes. Its stateful
+/// counterpart is ``sub``, see below.
+
+val gsub (#a: Type) (b: buffer a) (i: U32.t) (len: U32.t) : Ghost (buffer a)
+  (requires (U32.v i + U32.v len <= length b))
+  (ensures (fun y -> True))
+
+// goffset
+
+/// A buffer is live exactly at the same time as all of its sub-buffers.
+
+val live_gsub (#a: Type) (h: HS.mem) (b: buffer a) (i: U32.t) (len: U32.t) : Lemma
+  (requires (U32.v i + U32.v len <= length b))
+  (ensures (live h (gsub b i len) <==> live h b))
+  [SMTPatOr [
+    [SMTPat (live h (gsub b i len))];
+    [SMTPat (live h b); SMTPat (gsub b i len);]
+  ]]
+
+
+val gsub_is_null (#t: Type) (b: buffer t) (i: U32.t) (len: U32.t) : Lemma
+  (requires (U32.v i + U32.v len <= length b))
+  (ensures (g_is_null (gsub b i len) <==> g_is_null b))
+  [SMTPat (g_is_null (gsub b i len))]
+
+/// The length of a sub-buffer is exactly the one provided at ``gsub``.
+
+val len_gsub (#a: Type) (b: buffer a) (i: U32.t) (len': U32.t) : Lemma
+  (requires (U32.v i + U32.v len' <= length b))
+  (ensures (len (gsub b i len') == len'))
+  [SMTPatOr [
+    [SMTPat (len (gsub b i len'))];
+    [SMTPat (length (gsub b i len'))];
+  ]]
+
+val frameOf_gsub (#a: Type) (b: buffer a) (i: U32.t) (len : U32.t) : Lemma
+  (requires (U32.v i + U32.v len <= length b))
+  (ensures (frameOf (gsub b i len) == frameOf b))
+  [SMTPat (frameOf (gsub b i len))]
+
+val as_addr_gsub (#a: Type) (b: buffer a) (i: U32.t) (len : U32.t) : Lemma
+  (requires (U32.v i + U32.v len <= length b))
+  (ensures (as_addr (gsub b i len) == as_addr b))
+  [SMTPat (as_addr (gsub b i len))]
+
+val gsub_inj
+  (#t: Type)
+  (b1 b2: buffer t)
+  (i1 i2: U32.t)
+  (len1 len2: U32.t)
+: Lemma
+  (requires (U32.v i1 + U32.v len1 <= length b1 /\ U32.v i2 + U32.v len2 <= length b2 /\ gsub b1 i1 len1 == gsub b2 i2 len2))
+  (ensures (len1 == len2 /\ (b1 == b2 ==> i1 == i2) /\ ((i1 == i2 /\ length b1 == length b2) ==> b1 == b2)))
+
+/// Nesting two ``gsub`` collapses into one ``gsub``, transitively.
+
+val gsub_gsub (#a: Type) (b: buffer a) (i1: U32.t) (len1: U32.t) (i2: U32.t) (len2: U32.t) : Lemma
+  (requires (U32.v i1 + U32.v len1 <= length b /\ U32.v i2 + U32.v len2 <= U32.v len1))
+  (ensures (
+    U32.v i1 + U32.v len1 <= length b /\ U32.v i2 + U32.v len2 <= U32.v len1 /\
+    gsub (gsub b i1 len1) i2 len2 == gsub b (U32.add i1 i2) len2
+  ))
+  [SMTPat (gsub (gsub b i1 len1) i2 len2)]
+
+/// A buffer ``b`` is equal to its "largest" sub-buffer, at index 0 and
+/// length ``len b``.
+
+val gsub_zero_length (#a: Type) (b: buffer a) : Lemma
+  (b == gsub b 0ul (len b))
+
+
+/// The contents of a sub-buffer is the corresponding slice of the
+/// contents of its enclosing buffer.
+
+val as_seq_gsub (#a: Type) (h: HS.mem) (b: buffer a) (i: U32.t) (len: U32.t) : Lemma
+  (requires (U32.v i + U32.v len <= length b))
+  (ensures (as_seq h (gsub b i len) == Seq.slice (as_seq h b) (U32.v i) (U32.v i + U32.v len)))
+  [SMTPat (as_seq h (gsub b i len))]
+
